WIP current work on modelled.v

library/modelled.v
@@ -5,6 +5,90 @@ Require Import Psatz.
 Require Import List.
 Import ListNotations.
 
+Class Isomorphism (A B : Type) :=
+  { from : A -> B
+  ; to : B -> A
+  ; from_to : forall (x : A), to (from x) = x
+  ; to_from : forall (x : B), from (to x) = x
+  }.
+
+Instance Isomorphism_refl {A : Type} : Isomorphism A A.
+Proof.
+  refine {| from := id ; to := id ; from_to := _ ; to_from := _ |}; auto.
+Defined.
+
+Lemma Isomorphism_sym {A B : Type} : Isomorphism A B -> Isomorphism B A.
+Proof.
+  intro i.
+  exact {| from := to
+         ; to := from
+         ; from_to := to_from
+         ; to_from := from_to |}.
+Defined.
+
+Lemma Isomorphism_trans {A B C : Type} : Isomorphism A B -> Isomorphism B C -> Isomorphism A C.
+Proof.
+  intros [f1 t1 pf1 pt1] [f2 t2 pf2 pt2].
+  refine {| from := fun x => f2 (f1 x)
+          ; to := fun x => t1 (t2 x)
+          ; from_to := _
+          ; to_from := _ |};
+  intro; [rewrite pf2, pf1 | rewrite pt1, pt2]; auto.
+Defined.
+
+Lemma from_sym : forall A B `(M : Isomorphism A B),
+    @from A B M = @to B A (Isomorphism_sym M).
+Proof.
+  intros A B M; auto.
+Defined.
+
+Lemma to_sym : forall A B `(M : Isomorphism A B),
+    @to A B M = @from B A (Isomorphism_sym M).
+Proof.
+  intros A B M; auto.
+Defined.
+
+Lemma from_trans : forall A B C `(M1 : Isomorphism A B) `(M2 : Isomorphism B C),
+    forall (x : A), @from B C M2 (@from A B M1 x) = @from A C (Isomorphism_trans M1 M2) x .
+Proof.
+  intros A B C [f1 t1 pf1 pt1] [f2 t2 pf2 pt2] x; simpl; auto.
+Defined.
+
+
+Require Import Coq.Logic.FunctionalExtensionality.
+
+Lemma Isomorphism_dep_fn {A A' : Type} {B : A -> Type} {B' : A' -> Type} :
+  Isomorphism A A' ->
+  (forall (a : A) (a' : A'), Isomorphism A A' -> Isomorphism (B a) (B' a')) ->
+  Isomorphism (forall (a : A), B a) (forall (a' : A'), B' a').
+Proof.
+  intros.
+  econstructor.
+  instantiate (1 := ltac:(intros g a; exact (from (g (to a))))).
+  instantiate (1 := ltac:(intros g a'; exact (to (g (from a'))))).
+  all: intros; apply functional_extensionality_dep;
+       intro; rewrite ?from_to, ?to_from; auto.
+Defined.
+
+Lemma Isomorphism_fn {A A' B B' : Type} :
+  Isomorphism A A' -> Isomorphism B B' -> Isomorphism (A -> B) (A' -> B').
+Proof.
+  intros i1 i2.
+  exact (@Isomorphism_dep_fn A A' (fun _ => B) (fun _ => B') i1 (fun _ _ _ => i2)).
+Defined.
+
+(* Check f_equal. *)
+
+(* Lemma Isomorphism_f_equal {A B : Type} (F : Type -> Type) : *)
+(*   Isomorphism A B -> Isomorphism (F A) (F B). *)
+(* Proof. *)
+(*   intros [f t ft tf]. *)
+(*   refine {| from := fun (a : F A) => _; to := _; from_to := _; to_from := _ |}. *)
+(*   econstructor. *)
+(*   instantiate (1 := ltac:()). *)
+
+
+
 Ltac eq_refl_match :=
   match goal with
   | [ |- context[match ?x with | eq_refl => _ end] ] => destruct x
@@ -20,59 +104,13 @@ Ltac props x :=
   unfold id, eq_rect in *;
   clear P.
 
-Class Modelled (prim_type model_type : Type) :=
-  { model_to_prim : model_type -> prim_type
-  ; prim_to_model : prim_type -> model_type
-  ; prim_to_model_to_prim : forall (x : prim_type), model_to_prim (prim_to_model x) = x
-  ; model_to_prim_to_model : forall (x : model_type), prim_to_model (model_to_prim x) = x
-  }.
-
-Instance Modelled_same {A : Type} : Modelled A A.
-  refine (@Build_Modelled A A id id _ _); auto.
-Defined.
-
-Require Import Coq.Logic.FunctionalExtensionality.
-
-Instance Modelled_fn {A A' B B' : Type} :
-  Modelled A A' -> Modelled B B' -> Modelled (A -> B) (A' -> B').
-Proof.
-  intros ma mb.
-  pose (f1 (f : A -> B) := fun a' : A' => prim_to_model (f (model_to_prim a'))).
-  pose (f2 (f : A' -> B') := fun a : A => model_to_prim (f (prim_to_model a))).
-  refine (@Build_Modelled (A -> B) (A' -> B') f2 f1 _ _);
-  intros; unfold f1, f2; apply functional_extensionality;
-    intro; rewrite ?prim_to_model_to_prim, ?model_to_prim_to_model; auto.
-Defined.
-
-Instance Modelled_dep_fn {A A' : Type} {B : A -> Type} {B' : A' -> Type} :
-  Modelled A A' ->
-  (forall (a : A) (a' : A'), Modelled A A' -> Modelled (B a) (B' a')) ->
-  Modelled (forall (a : A), B a) (forall (a' : A'), B' a').
-Proof.
-  intros ma f.
-  econstructor.
-  Unshelve.
-  3: intros g a; exact (model_to_prim (g (prim_to_model a))).
-  3: intros g a'; exact (prim_to_model (g (model_to_prim a'))).
-  * intros x.
-    apply (functional_extensionality_dep _ x).
-    intro a.
-    rewrite !prim_to_model_to_prim.
-    auto.
-  * intros x.
-    apply (functional_extensionality_dep _ x).
-    intro a'.
-    rewrite !model_to_prim_to_model.
-    auto.
-Defined.
-
 Require Import VeriFFI.library.meta.
 
 (* opaque and transparent *)
 Inductive annotated : Type :=
 | TYPEPARAM : (forall (A : Type) `{Rep A}, annotated) -> annotated
 | OPAQUE : forall (prim_type model_type : Type)
-                    `{Modelled prim_type model_type},
+                    `{Isomorphism prim_type model_type},
                     (option (prim_type -> annotated)) ->
                     annotated
 | TRANSPARENT : forall (A : Type) `{Rep A}, (option (A -> annotated)) -> annotated.
@@ -102,7 +140,7 @@ Fixpoint to_model_fn_type (r : annotated) : Type :=
   | OPAQUE pt mt M o =>
       match o with
       | None => mt
-      | Some fp => forall (m : mt), to_model_fn_type (fp (model_to_prim m))
+      | Some fp => forall (m : mt), to_model_fn_type (fp (@to pt mt M m))
       end
   | TRANSPARENT t R o =>
       match o with
@@ -126,10 +164,825 @@ destruct a as [f|prim_type model_type M|A R o]; simpl in ft, mt.
 * exact (forall (A : Type), model_spec_aux (f A Rep_any) (ft A) (mt A)).
 * destruct o as [pf|].
   - refine (forall (x : prim_type), model_spec_aux (pf x) (ft x) _).
-    pose (m := mt (prim_to_model x)).
-    rewrite prim_to_model_to_prim in m.
+    pose (m := mt (@from prim_type model_type M x)).
+    rewrite from_to in m.
     exact m.
-  - exact (ft = model_to_prim mt).
+  - exact (ft = to mt).
+* destruct o as [pf|].
+  - exact (forall (x : A), model_spec_aux (pf x) (ft x) (mt x)).
+  - exact (ft = mt).
+Defined.
+
+Definition model_spec (ep : extern_properties) : Prop :=
+  model_spec_aux (type_desc ep) (prim_fn ep) (model_fn ep).
+
+Module IntVerification.
+
+Module Type UInt63.
+  Axiom t : Type.
+  Axiom from_Z : Z -> t.
+  Axiom to_Z : t -> Z.
+  Axiom add : t -> t -> t.
+  Axiom mul : t -> t -> t.
+End UInt63.
+
+(* Axiom VSU : Type. *)
+(* Axiom int63_vsu : VSU. *)
+(* Axiom lift : forall {A : Type}, A -> VSU -> string -> A. *)
+
+Module FM <: UInt63.
+  Definition t := {z : Z | 0 <= z < 2^63}%Z.
+  Definition from_Z (z : Z) : t.
+    exists (Z.modulo z (2^63)).
+    apply Z_mod_lt.
+    constructor.
+  Defined.
+
+  Definition to_Z (z : t) : Z := proj1_sig z.
+  Definition add (x y : t) : t.
+    destruct x as [xz x_pf], y as [yz y_pf].
+    exists ((xz + yz) mod (2^63))%Z.
+    split.
+    * destruct x_pf as [x_pf1 _], y_pf as [y_pf1 _].
+      apply Z_mod_nonneg_nonneg.
+      apply Z.add_nonneg_nonneg.
+      assumption. assumption.
+      apply Pos2Z.is_nonneg.
+    * apply Z.mod_pos_bound.
+      constructor.
+  Defined.
+
+  Definition mul (x y : t) : t.
+    destruct x as [xz x_pf], y as [yz y_pf].
+    exists ((xz * yz) mod (2^63))%Z.
+    split.
+    * destruct x_pf as [x_pf1 _], y_pf as [y_pf1 _].
+      apply Z_mod_nonneg_nonneg.
+      apply Z.mul_nonneg_nonneg.
+      assumption. assumption.
+      apply Pos2Z.is_nonneg.
+    * apply Z.mod_pos_bound.
+      constructor.
+  Defined.
+End FM.
+
+Module C : UInt63.
+  Axiom t : Type.
+  Axiom from_Z : Z -> t.
+  Axiom to_Z : t -> Z.
+  Axiom add : t -> t -> t.
+  Axiom mul : t -> t -> t.
+End C.
+
+Module UInt63_Proofs.
+
+  Require Import JMeq.
+  (* Axiom P_pf : forall (T : Type) (P : (T -> FM.t) -> Prop) , *)
+  (*     (C.t = FM.t -> JMeq C.add FM.add -> JMeq C.mul FM.mul -> JMeq C.from_Z FM.from_Z -> JMeq C.to_Z FM.to_Z -> *)
+  (*      forall x x', (forall i, JMeq (x i) (x' i)) -> (P x = P x')). *)
+
+
+  (* Axiom P_pf : forall (T : Type) (P : (T -> C.t) -> Prop) (P' : (T -> FM.t) -> Prop), *)
+  (*     (C.t = FM.t -> JMeq C.add FM.add -> JMeq C.mul FM.mul -> JMeq C.from_Z FM.from_Z -> JMeq C.to_Z FM.to_Z -> *)
+  (*      forall x x', (forall i, JMeq (x i) (x' i)) -> (P x = P' x')). *)
+
+
+  Definition Rep_Z : Rep Z. Admitted.
+  Axiom Isomorphism_t : Isomorphism C.t FM.t.
+
+  Definition from_Z_ep : extern_properties :=
+    {| type_desc :=
+        @TRANSPARENT Z Rep_Z
+           (Some (fun z => @OPAQUE _ _ Isomorphism_t None))
+     ; prim_fn := C.from_Z
+     ; model_fn := FM.from_Z
+     ; c_name := "int63_from_Z"
+     |}.
+
+  Definition to_Z_ep : extern_properties :=
+    {| type_desc :=
+        @OPAQUE _ _ Isomorphism_t
+           (Some (fun z => @TRANSPARENT Z Rep_Z None))
+     ; prim_fn := C.to_Z
+     ; model_fn := FM.to_Z
+     ; c_name := "int63_to_Z"
+     |}.
+
+  Definition add_ep : extern_properties :=
+    {| type_desc :=
+          @OPAQUE _ _ Isomorphism_t
+            (Some (fun i =>
+              @OPAQUE _ _ Isomorphism_t
+                (Some (fun i => @OPAQUE _ _ Isomorphism_t None))))
+     ; prim_fn := C.add
+     ; model_fn := FM.add
+     ; c_name := "int63_add"
+     |}.
+
+  Definition mul_ep : extern_properties :=
+    {| type_desc :=
+          @OPAQUE _ _ Isomorphism_t
+            (Some (fun i =>
+              @OPAQUE _ _ Isomorphism_t
+                (Some (fun i => @OPAQUE _ _ Isomorphism_t None))))
+     ; prim_fn := C.mul
+     ; model_fn := FM.mul
+     ; c_name := "int63_mul"
+     |}.
+
+  Axiom from_Z_properties : model_spec from_Z_ep.
+  Axiom to_Z_properties : model_spec to_Z_ep.
+  Axiom add_properties : model_spec add_ep.
+  Axiom mul_properties : model_spec mul_ep.
+
+  Lemma seven : C.to_Z (C.add (C.from_Z 3%Z) (C.from_Z 4%Z)) = 7%Z.
+  Proof.
+
+    Print model_spec.
+    Print model_spec_aux.
+
+  let P := fresh in
+  pose proof from_Z_properties as P;
+  hnf in P;
+  simpl in P;
+  rewrite !P;
+  unfold id, eq_rect in *.
+
+    props from_Z_properties.
+    props to_Z_properties.
+    props add_properties.
+    repeat eq_refl_match.
+    rewrite !from_to, !to_from.
+    unfold FM.to_Z, FM.add, FM.from_Z.
+    simpl.
+    rewrite Z.mod_small.
+    auto.
+    lia.
+  Qed.
+
+  Lemma add_assoc : forall (x y z : Z),
+    C.to_Z (C.add (C.from_Z x) (C.add (C.from_Z y) (C.from_Z z))) =
+    C.to_Z (C.add (C.add (C.from_Z x) (C.from_Z y)) (C.from_Z z)).
+  Proof.
+    intros x y z.
+    props from_Z_properties.
+    props to_Z_properties.
+    props add_properties.
+    repeat eq_refl_match.
+    rewrite !from_to, !to_from.
+    unfold FM.add, FM.from_Z, FM.to_Z.
+    simpl.
+    rewrite <- !(Z.add_mod y z).
+    rewrite <- !(Z.add_mod x y).
+    rewrite <- !(Z.add_mod).
+    f_equal.
+    apply Z.add_assoc.
+    all: lia.
+  Qed.
+
+  Lemma mul_add_distr_l : forall (x y z : Z),
+    C.to_Z (C.mul (C.from_Z x) (C.add (C.from_Z y) (C.from_Z z))) =
+    C.to_Z (C.add (C.mul (C.from_Z x) (C.from_Z y)) (C.mul (C.from_Z x) (C.from_Z z))).
+  Proof.
+    intros x y z.
+    props from_Z_properties.
+    props to_Z_properties.
+    props add_properties.
+    props mul_properties.
+    repeat eq_refl_match.
+    rewrite !from_to, !to_from.
+    unfold FM.mul, FM.add, FM.from_Z, FM.to_Z.
+    simpl.
+    pose (y' := Z.modulo y (Z.pow_pos 2 63)); fold y'.
+    pose (z' := Z.modulo z (Z.pow_pos 2 63)); fold z'.
+    rewrite <- Zplus_mod.
+    rewrite <- Z.mul_add_distr_l.
+    rewrite Zmult_mod_idemp_r.
+    auto.
+  Qed.
+
+  Lemma mul_add_distr_r : forall (x y z : Z),
+    C.to_Z (C.mul (C.add (C.from_Z x) (C.from_Z y)) (C.from_Z z)) =
+    C.to_Z (C.add (C.mul (C.from_Z x) (C.from_Z z)) (C.mul (C.from_Z y) (C.from_Z z))).
+  Proof.
+    intros x y z.
+    props from_Z_properties.
+    props to_Z_properties.
+    props add_properties.
+    props mul_properties.
+    repeat eq_refl_match.
+    rewrite !from_to, !to_from.
+    unfold FM.mul, FM.add, FM.from_Z, FM.to_Z.
+    simpl.
+    pose (x' := Z.modulo y (Z.pow_pos 2 63)); fold x'.
+    pose (y' := Z.modulo y (Z.pow_pos 2 63)); fold y'.
+    pose (z' := Z.modulo z (Z.pow_pos 2 63)); fold z'.
+    rewrite <- Zplus_mod.
+    rewrite <- Z.mul_add_distr_r.
+    rewrite Zmult_mod_idemp_l.
+    auto.
+  Qed.
+
+End UInt63_Proofs.
+
+End IntVerification.
+
+Module ArrayVerification.
+
+Module Type Element.
+  Axiom t : Type.
+End Element.
+
+Module Type Array (E : Element).
+  Axiom arrays : Type.
+  Definition ST (S : Type) (A : Type) : Type := arrays -> A * arrays.
+  Axiom pure : forall {S A}, A -> ST S A.
+  Axiom bind : forall {S A B}, ST S A -> (A -> ST S B) -> ST S B.
+  Axiom runST : forall {A}, (forall S, ST S A) -> A.
+  Axiom array : Type -> Type.
+  Axiom new : forall {S}, nat -> E.t -> ST S (array S).
+  Axiom set : forall {S}, array S -> nat -> E.t -> ST S unit.
+  Axiom get : forall {S}, array S -> nat -> ST S (option E.t).
+  Axiom delete : forall {S}, array S -> ST S unit.
+End Array.
+
+Module FM (E : Element) <: Array E.
+  Definition array (S : Type) : Type := nat.
+  Definition arrays := list (list E.t).
+  Definition ST (S : Type) (A : Type) : Type := arrays -> A * arrays.
+  Definition pure {S A} (a : A) : ST S A := fun s => (a, s).
+  Definition bind {S A B} (m : ST S A) (f : A -> ST S B) : ST S B :=
+    fun s => f (fst (m s)) (snd (m s)).
+    (* fun s => let '(a, s') := m s in f a s'. *)
+  Definition runST {A} (f : forall S, ST S A) : A :=
+    fst (f unit nil).
+  Definition new {S} (len : nat) (fill : E.t) : ST S (array S) :=
+    let xs := repeat fill len in
+    fun s => (length s, s ++ [xs]).
+
+  (* Look at canon.replace_nth, invariants.replace_nth, sepalg_list.replace for lemmas *)
+  Definition set {S} (arr : array S) (index : nat) (elt : E.t) : ST S unit :=
+    let fix replace (index : nat) (l : list E.t) : list E.t :=
+      match index, l with
+      | _, nil => nil
+      | O, cons x xs => cons elt xs
+      | S n, cons x xs => cons x (replace n xs)
+      end in
+    let fix aux (s : arrays) (arr : array S) : arrays :=
+      match arr, s with
+      | _, nil => nil
+      | O, cons x xs => cons (replace index x) xs
+      | S n, cons x xs => cons x (aux xs n)
+      end
+    in fun s => (tt, aux s arr).
+
+  Definition get {S} (arr : array S) (index : nat) : ST S (option E.t) :=
+    fun s : arrays =>
+      match nth_error s arr with
+      | None => (None, s)
+      | Some l => (nth_error l index, s)
+      end.
+
+  Definition delete {S} (arr : array S) : ST S unit :=
+    let fix aux (s : arrays) (arr : array S) : arrays :=
+      match arr, s with
+      | _, nil => nil
+      | O, cons x xs => cons nil xs
+      | S n, cons x xs => cons x (aux xs n)
+      end
+    in fun s => (tt, aux s arr).
+End FM.
+
+Module C (E : Element) : Array E.
+  Axiom arrays : Type.
+  Definition ST (S : Type) (A : Type) : Type := arrays -> A * arrays.
+  Axiom pure : forall {S A}, A -> ST S A.
+  Axiom bind : forall {S A B}, ST S A -> (A -> ST S B) -> ST S B.
+  Axiom runST : forall {A}, (forall S, ST S A) -> A.
+  Axiom array : Type -> Type.
+  Axiom new : forall {S}, nat -> E.t -> ST S (array S).
+  Axiom set : forall {S}, array S -> nat -> E.t -> ST S unit.
+  Axiom get : forall {S}, array S -> nat -> ST S (option E.t).
+  Axiom delete : forall {S}, array S -> ST S unit.
+End C.
+
+Module Array_Proofs.
+  Module E.
+    Definition t := bool.
+  End E.
+  Module FM := FM E.
+  Module C := C E.
+
+  Definition Rep_nat : Rep nat. Admitted.
+  Definition Rep_t : Rep E.t. Admitted.
+
+  Variable Isomorphism_array : forall {S}, Isomorphism (C.array S) (FM.array S).
+  Variable Isomorphism_arrays : Isomorphism (C.arrays) (FM.arrays).
+
+  Definition Isomorphism_ST
+             {S A A' : Type} (I : Isomorphism A A') : Isomorphism (C.ST S A) (FM.ST S A').
+    destruct I as [f t pf pt].
+    destruct (@Isomorphism_array S) as [f' t' pf' pt'].
+    unfold FM.ST, C.ST.
+    apply Isomorphism_fn.
+    apply Isomorphism_arrays.
+    Admitted.
+
+
+
+
+
+  (* Axiom Isomorphism_ST : forall {S A A'}, Isomorphism A A' -> Isomorphism (C.ST S A) (FM.ST S A'). *)
+  Axiom Isomorphism_ST_inj : forall {S A A'}, Isomorphism (C.ST S A) (FM.ST S A') -> Isomorphism A A'.
+
+  Definition pure_ep : extern_properties :=
+    {| type_desc :=
+      @TYPEPARAM (fun (S : Type) `{Rep_S : Rep S} =>
+        @TYPEPARAM (fun (A : Type) `{Rep_A : Rep A} =>
+          @TRANSPARENT A Rep_A (Some (fun arr =>
+            @OPAQUE (C.ST S A) (FM.ST S A) (Isomorphism_ST _) None))))
+     ; prim_fn := @C.pure
+     ; model_fn := @FM.pure
+     ; c_name := "st_pure"
+     |}.
+
+  Definition bind_ep : extern_properties :=
+    {| type_desc :=
+      @TYPEPARAM (fun (S : Type) `{Rep_S : Rep S} =>
+        @TYPEPARAM (fun (A : Type) `{Rep_A : Rep A} =>
+          @TYPEPARAM (fun (B : Type) `{Rep_B : Rep B} =>
+            @OPAQUE (C.ST S A) (FM.ST S A) (Isomorphism_ST _) (Some (fun m =>
+              @OPAQUE (A -> C.ST S B) (A -> FM.ST S B) (Isomorphism_fn _ (Isomorphism_ST _)) (Some (fun f =>
+                @OPAQUE (C.ST S B) (FM.ST S B) (Isomorphism_ST _) None)))))))
+     ; prim_fn := @C.bind
+     ; model_fn := @FM.bind
+     ; c_name := "st_bind"
+     |}.
+
+  Definition runST_ep : extern_properties :=
+    {| type_desc :=
+      @TYPEPARAM (fun (A : Type) `{Rep_A : Rep A} =>
+          @OPAQUE (forall (S : Type), C.ST S A) (forall (S : Type), FM.ST S A)
+                  (@Isomorphism_dep_fn Type Type (fun S => C.ST S A) (fun S => FM.ST S A) _
+                                    (fun s s' m => @Isomorphism_ST _ A A _)) (Some (fun f =>
+            @TRANSPARENT A Rep_A None)))
+     ; prim_fn := @C.runST
+     ; model_fn := @FM.runST
+     ; c_name := "st_runST"
+     |}.
+
+  Definition new_ep : extern_properties :=
+    {| type_desc :=
+      @TYPEPARAM (fun (S : Type) `{Rep_S : Rep S} =>
+        @TRANSPARENT nat Rep_nat (Some (fun n =>
+          @TRANSPARENT E.t Rep_t (Some (fun a =>
+            @OPAQUE (C.ST S (C.array S)) (FM.ST S (FM.array S))
+                    (Isomorphism_ST Isomorphism_array) None)))))
+     ; prim_fn := @C.new
+     ; model_fn := @FM.new
+     ; c_name := "array_new"
+     |}.
+
+  Definition set_ep : extern_properties :=
+    {| type_desc :=
+      @TYPEPARAM (fun (S : Type) `{Rep_S : Rep S} =>
+        @OPAQUE (C.array S) (FM.array S) Isomorphism_array (Some (fun arr =>
+          @TRANSPARENT nat Rep_nat (Some (fun n =>
+            @TRANSPARENT E.t Rep_t (Some (fun a =>
+              @OPAQUE (C.ST S unit) (FM.ST S unit) (Isomorphism_ST _) None)))))))
+     ; prim_fn := @C.set
+     ; model_fn := @FM.set
+     ; c_name := "array_set"
+     |}.
+
+  Definition get_ep : extern_properties :=
+    {| type_desc :=
+      @TYPEPARAM (fun (S : Type) `{Rep_S : Rep S} =>
+        @OPAQUE (C.array S) (FM.array S) Isomorphism_array (Some (fun arr =>
+          @TRANSPARENT nat Rep_nat (Some (fun n =>
+            @OPAQUE (C.ST S (option E.t)) (FM.ST S (option E.t)) (Isomorphism_ST _) None)))))
+     ; prim_fn := @C.get
+     ; model_fn := @FM.get
+     ; c_name := "array_get"
+     |}.
+
+  Definition delete_ep : extern_properties :=
+    {| type_desc :=
+      @TYPEPARAM (fun (S : Type) `{Rep_S : Rep S} =>
+        @OPAQUE (C.array S) (FM.array S) Isomorphism_array (Some (fun arr =>
+          @OPAQUE (C.ST S unit) (FM.ST S unit) (Isomorphism_ST _) None)))
+     ; prim_fn := @C.delete
+     ; model_fn := @FM.delete
+     ; c_name := "array_delete"
+     |}.
+
+  Axiom pure_properties : model_spec pure_ep.
+  Axiom bind_properties : model_spec bind_ep.
+  Axiom runST_properties : model_spec runST_ep.
+  Axiom new_properties : model_spec new_ep.
+  Axiom set_properties : model_spec set_ep.
+  Axiom get_properties : model_spec get_ep.
+  Axiom delete_properties : model_spec delete_ep.
+
+  Ltac prim_rewrites :=
+    repeat eq_refl_match;
+    rewrite ?from_to, ?to_from.
+
+  (* Definition actions_equiv {S A : Type} (x y : FM.ST S A) : Prop := *)
+  (*   forall s, x s = y s. *)
+  (* Set Printing All. *)
+  (* Print actions_equiv. *)
+
+  (* Axiom runST_equiv : forall A (x y : forall (S : Type), FM.ST S A), *)
+  (*     x = y -> *)
+  (*     FM.runST x = FM.runST y. *)
+
+
+  Arguments from A B {_}.
+  Arguments to A B {_}.
+
+  Axiom array_eq : forall S, C.array S = FM.array S.
+  (* Lemma from_eq : *)
+  (*   forall A B x, *)
+  (*     A = B -> *)
+  (*     from A B x = x. *)
+
+  Lemma Isomorphism_FMST {A B : Type} : Isomorphism A B -> Isomorphism (FM.ST unit A) (FM.ST unit B).
+  Proof.
+    intros [f t ft tf].
+    econstructor.
+    Unshelve.
+    3: { intros a x. specialize (a x).
+         exact (f (fst a), (snd a)).}
+    3: { intros a x. specialize (a x).
+         exact (t (fst a), (snd a)).}
+    simpl. intros. apply functional_extensionality. intros. rewrite ?ft, ?tf. destruct (x x0). auto.
+    simpl. intros. apply functional_extensionality. intros. rewrite ?ft, ?tf. destruct (x x0). auto.
+  Defined.
+
+
+  (* Lemma from_eq : *)
+  (*   forall A B x, *)
+  (*     A = B -> *)
+  (*     forall (I1 : Isomorphism A B) (I2 : Isomorphism (FM.ST unit B) (FM.ST unit A)), *)
+  (*       I2 = Isomorphism_sym (Isomorphism_FMST I1) -> *)
+  (*   (@from A B I1 (fst (@from (FM.ST unit B) (FM.ST unit A) I2 x []))) = fst (x []). *)
+  (* Proof. *)
+  (*   intros A B X eq I1 I2 Ieq. *)
+  (*   subst. *)
+  (* Admitted. *)
+  (*   unfold fst. *)
+  (*   unfold fst. *)
+  (* Abort. *)
+
+  Require Import JMeq.
+
+  Require Import Coq.Logic.FunctionalExtensionality.
+  Require Import Coq.Logic.JMeq.
+
+  Theorem jmeq_funext
+    A (P : A -> Type) (Q : A -> Type)
+    (f : forall a, P a)(g : forall a, Q a)
+    (h : forall a, JMeq (f a) (g a)) : JMeq f g.
+  Proof.
+    assert (pq_eq : P = Q).
+      apply functional_extensionality.
+      exact (fun a => match (h a) with JMeq_refl => eq_refl end).
+    induction pq_eq.
+    assert (fg_eq : f = g).
+      apply functional_extensionality_dep.
+      exact (fun a => JMeq_rect (fun ga => f a = ga) eq_refl (h a)).
+    induction fg_eq.
+    exact JMeq_refl.
+  Qed.
+
+
+  Axiom runST_pf : forall {A : Type}
+                          {f : forall (S : Type), C.ST S A}
+                          {f' : forall (S : Type), FM.ST S A},
+   (forall (eq_array : forall {S}, (C.array S) = (FM.array S))
+           (eq_arrays : C.arrays = FM.arrays), JMeq f f') ->
+   (C.runST f) = (FM.runST f').
+
+  Lemma set_get :
+    forall {S : Type} (n len : nat) (bound : n < len) (to_set to_fill : E.t),
+      (C.runST (fun _ => C.bind (C.new len to_fill) (fun arr => C.bind (C.set arr n to_set) (fun _ => C.get arr n))))
+        =
+      (C.runST (fun _ => C.pure (Some to_set))).
+  Proof.
+
+    (* Set Printing Implicit. *)
+    (* Unset Printing Notations. *)
+
+
+    intros S n len bound to_set to_fill.
+
+    erewrite runST_pf.
+    instantiate (1 := fun _ => FM.bind (FM.new len to_fill) (fun arr => FM.bind (FM.set arr n to_set) (fun _ => FM.get arr n))).
+    erewrite runST_pf.
+    instantiate (1 := (fun _ => FM.pure (Some to_set))).
+
+
+    admit.
+
+
+    intros array_eq arrays_eq.
+    apply jmeq_funext.
+    intro A.
+    admit.
+
+    intros array_eq arrays_eq.
+    apply jmeq_funext.
+    intro A.
+    admit.
+
+
+
+
+
+
+
+
+
+
+    props runST_properties.
+    prim_rewrites.
+    unfold FM.runST.
+
+    props bind_properties.
+    props pure_properties.
+    props new_properties.
+    unfold FM.bind, FM.pure.
+    prim_rewrites.
+
+    props bind_properties.
+    unfold FM.bind.
+    prim_rewrites.
+
+    props set_properties.
+    prim_rewrites.
+
+    props get_properties.
+    prim_rewrites.
+
+    unfold fst at 4.
+
+    rewrite !to_sym.
+    rewrite !from_trans.
+    rewrite from_eq.
+    3: {
+      Set Printing All.
+      Check (@Isomorphism_ST unit (C.array unit) (C.array unit) (@Isomorphism_refl (C.array unit))).
+      unfold Isomorphism_sym.
+      simpl.
+      Set Printing All.
+      Check (@Isomorphism_ST unit (C.array unit) (C.array unit) (@Isomorphism_refl (C.array unit))).
+      Check (@Isomorphism_refl (FM.ST unit (FM.array unit))).
+      replace (@Isomorphism_ST unit (C.array unit) (C.array unit) (@Isomorphism_refl (C.array unit)))
+         with (@Isomorphism_refl (FM.ST unit (FM.array unit))).
+
+    }
+
+
+
+    Set Printing All.
+
+    (* rewrite array_eq. *)
+
+    (* Set Printing Implicit. *)
+
+    unfold FM.new, FM.set, FM.get.
+    unfold repeat.
+
+    simpl.
+    all: try auto.
+
+
+    rewrite !to_sym.
+    rewrite !from_trans.
+
+
+
+    Unset Printing Implicit.
+
+
+    (* rest of the proof is just about the functional model *)
+    Set Printing All.
+    Check (@FM.new unit len to_fill).
+    rewrite ?from_to, ?to_from.
+    unfold FM.new.
+    rewrite ?from_to, ?to_from.
+
+    unfold from.
+
+    assert (forall (x : FM.ST S nat), to (from x) = x).
+    intros. prim_rewrites. auto.
+
+
+    rewrite (H (fun s : FM.arrays => (length s, s ++ [repeat to_fill len]))).
+    rewrite !to_from.
+    unfold FM.get, FM.set, FM.new.
+    simpl.
+    prim_rewrites.
+
+
+  Qed.
+
+End Array_Proofs.
+
+End ArrayVerification.
+Require Import String.
+
+Require Import ZArith.
+Require Import Psatz.
+Require Import List.
+Import ListNotations.
+
+
+Require Import Coq.Logic.FinFun.
+Require Import Coq.Relations.Relation_Definitions.
+Require Import Coq.Relations.Relation_Operators.
+Require Import Coq.Program.Basics.
+Require Import Coq.Program.Combinators.
+Require Import Setoid.
+
+
+Inductive P {A : Type} : A -> Prop :=
+| MkP : forall a, P a.
+
+Class Isomorphism (A B : Type) : Type :=
+  { from : A -> B
+  ; to : B -> A
+  ; from_to : forall (x : A), to (from x) = x
+  ; to_from : forall (x : B), from (to x) = x
+  }.
+
+(* Require Import Coq.Logic.FinFun. *)
+(* Require Import Coq.Relations.Relation_Definitions. *)
+(* Require Import Coq.Relations.Relation_Operators. *)
+(* Require Import Coq.Program.Basics. *)
+(* Require Import Coq.Program.Combinators. *)
+(* Require Import Setoid. *)
+
+Instance Isomorphism_refl {A : Type} : Isomorphism A A.
+Proof.
+  eapply {| from := id ; to := id ; from_to := ltac:(auto) ; to_from := ltac:(auto) |}.
+Defined.
+
+Lemma Isomorphism_sym {A B : Type} `(I : Isomorphism A B) : Isomorphism B A.
+Proof.
+  destruct I as [f t ft tf].
+  eapply {| from := t ; to := f ; from_to := tf ; to_from := ft |}.
+Defined.
+
+Lemma Isomorphism_trans {A B C : Type}
+      `(I1 : Isomorphism A B)
+      `(I2 : Isomorphism B C) : Isomorphism A C.
+Proof.
+  destruct I1 as [f1 t1 ft1 tf1].
+  destruct I2 as [f2 t2 ft2 tf2].
+  eapply {| from := fun x => f2 (f1 x)
+          ; to := fun x => t1 (t2 x)
+          ; from_to := _
+          ; to_from := _|}.
+
+  Unshelve.
+  intros; simpl; rewrite ft2, ft1; auto.
+  intros; simpl; rewrite tf1, tf2; auto.
+Defined.
+
+Lemma from_sym : forall A B `(M : Isomorphism A B),
+    @from A B M = @to B A (Isomorphism_sym M).
+Proof.
+  intros A B M; destruct M; auto.
+Defined.
+
+Lemma to_sym : forall A B `(M : Isomorphism A B),
+    @to A B M = @from B A (Isomorphism_sym M).
+Proof.
+  intros A B M; destruct M; auto.
+Defined.
+
+Lemma from_trans : forall A B C `(M1 : Isomorphism A B) `(M2 : Isomorphism B C),
+    forall (x : A), @from B C M2 (@from A B M1 x) = @from A C (Isomorphism_trans M1 M2) x .
+Proof.
+  intros A B C [f1 t1 pf1 pt1] [f2 t2 pf2 pt2] x; simpl; auto.
+Defined.
+
+
+Require Import Coq.Logic.FunctionalExtensionality.
+
+Lemma Isomorphism_dep_fn {A A' : Type} {B : A -> Type} {B' : A' -> Type} :
+  Isomorphism A A' ->
+  (forall (a : A) (a' : A'), Isomorphism A A' -> Isomorphism (B a) (B' a')) ->
+  Isomorphism (forall (a : A), B a) (forall (a' : A'), B' a').
+Proof.
+  intros.
+  econstructor.
+  instantiate (1 := ltac:(intros g a; exact (from (g (to a))))).
+  instantiate (1 := ltac:(intros g a'; exact (to (g (from a'))))).
+  all: intros; apply functional_extensionality_dep;
+       intro; rewrite ?from_to, ?to_from; auto.
+Defined.
+
+Lemma Isomorphism_fn {A A' B B' : Type} :
+  Isomorphism A A' -> Isomorphism B B' -> Isomorphism (A -> B) (A' -> B').
+Proof.
+  intros i1 i2.
+  exact (@Isomorphism_dep_fn A A' (fun _ => B) (fun _ => B') i1 (fun _ _ _ => i2)).
+Defined.
+
+Check f_equal.
+
+(* Lemma Isomorphism_f_equal {A B : Type} (F : Type -> Type) : *)
+(*   Isomorphism A B -> Isomorphism (F A) (F B). *)
+(* Proof. *)
+(*   intros [f t ft tf]. *)
+(*   refine {| from := fun (a : F A) => _; to := _; from_to := _; to_from := _ |}. *)
+(*   econstructor. *)
+(*   instantiate (1 := ltac:()). *)
+
+
+
+Ltac eq_refl_match :=
+  match goal with
+  | [ |- context[match ?x with | eq_refl => _ end] ] => destruct x
+  (* | [ _ : context[match ?x with | eq_refl => _ end] |- _] => destruct x *)
+  end.
+
+Ltac props x :=
+  let P := fresh in
+  pose proof x as P;
+  hnf in P;
+  simpl in P;
+  rewrite !P;
+  unfold id, eq_rect in *;
+  clear P.
+
+Require Import VeriFFI.library.meta.
+
+(* opaque and transparent *)
+Inductive annotated : Type :=
+| TYPEPARAM : (forall (A : Type) `{Rep A}, annotated) -> annotated
+| OPAQUE : forall (prim_type model_type : Type)
+                    `{Isomorphism prim_type model_type},
+                    (option (prim_type -> annotated)) ->
+                    annotated
+| TRANSPARENT : forall (A : Type) `{Rep A}, (option (A -> annotated)) -> annotated.
+
+Definition Rep_Z : Rep Z. Admitted.
+
+Theorem Rep_any : forall {A : Type}, Rep A. Admitted.
+
+Fixpoint to_prim_fn_type (r : annotated) : Type :=
+  match r with
+  | TYPEPARAM f => forall (A : Type), to_prim_fn_type (f A Rep_any)
+  | OPAQUE pt mt M o =>
+      match o with
+      | None => pt
+      | Some fp => forall (p : pt), to_prim_fn_type (fp p)
+      end
+  | TRANSPARENT t R o =>
+      match o with
+      | None => t
+      | Some f => forall (x : t), to_prim_fn_type (f x)
+      end
+  end.
+
+Fixpoint to_model_fn_type (r : annotated) : Type :=
+  match r with
+  | TYPEPARAM f => forall (A : Type), to_model_fn_type (f A Rep_any)
+  | OPAQUE pt mt M o =>
+      match o with
+      | None => mt
+      | Some fp => forall (m : mt), to_model_fn_type (fp (@to pt mt M m))
+      end
+  | TRANSPARENT t R o =>
+      match o with
+      | None => t
+      | Some f => forall (x : t), to_model_fn_type (f x)
+      end
+  end.
+
+Record extern_properties :=
+  { type_desc : annotated
+  ; prim_fn : to_prim_fn_type type_desc
+  ; model_fn : to_model_fn_type type_desc
+  ; c_name : string
+  }.
+
+Fixpoint model_spec_aux
+         (a : annotated)
+         (ft : to_prim_fn_type a)
+         (mt : to_model_fn_type a) {struct a} : Prop.
+destruct a as [f|prim_type model_type M|A R o]; simpl in ft, mt.
+* exact (forall (A : Type), model_spec_aux (f A Rep_any) (ft A) (mt A)).
+* destruct o as [pf|].
+  - refine (forall (x : prim_type), model_spec_aux (pf x) (ft x) _).
+    pose (m := mt (@from prim_type model_type M x)).
+    rewrite from_to in m.
+    exact m.
+  - exact (ft = to mt).
 * destruct o as [pf|].
   - exact (forall (x : A), model_spec_aux (pf x) (ft x) (mt x)).
   - exact (ft = mt).
@@ -198,12 +1051,12 @@ End C.
 
 Module UInt63_Proofs.
   Definition Rep_Z : Rep Z. Admitted.
-  Axiom Modelled_t : Modelled C.t FM.t.
+  Axiom Isomorphism_t : Isomorphism C.t FM.t.
 
   Definition from_Z_ep : extern_properties :=
     {| type_desc :=
         @TRANSPARENT Z Rep_Z
-           (Some (fun z => @OPAQUE _ _ Modelled_t None))
+           (Some (fun z => @OPAQUE _ _ Isomorphism_t None))
      ; prim_fn := C.from_Z
      ; model_fn := FM.from_Z
      ; c_name := "int63_from_Z"
@@ -211,7 +1064,7 @@ Module UInt63_Proofs.
 
   Definition to_Z_ep : extern_properties :=
     {| type_desc :=
-        @OPAQUE _ _ Modelled_t
+        @OPAQUE _ _ Isomorphism_t
            (Some (fun z => @TRANSPARENT Z Rep_Z None))
      ; prim_fn := C.to_Z
      ; model_fn := FM.to_Z
@@ -220,10 +1073,10 @@ Module UInt63_Proofs.
 
   Definition add_ep : extern_properties :=
     {| type_desc :=
-          @OPAQUE _ _ Modelled_t
+          @OPAQUE _ _ Isomorphism_t
             (Some (fun i =>
-              @OPAQUE _ _ Modelled_t
-                (Some (fun i => @OPAQUE _ _ Modelled_t None))))
+              @OPAQUE _ _ Isomorphism_t
+                (Some (fun i => @OPAQUE _ _ Isomorphism_t None))))
      ; prim_fn := C.add
      ; model_fn := FM.add
      ; c_name := "int63_add"
@@ -231,10 +1084,10 @@ Module UInt63_Proofs.
 
   Definition mul_ep : extern_properties :=
     {| type_desc :=
-          @OPAQUE _ _ Modelled_t
+          @OPAQUE _ _ Isomorphism_t
             (Some (fun i =>
-              @OPAQUE _ _ Modelled_t
-                (Some (fun i => @OPAQUE _ _ Modelled_t None))))
+              @OPAQUE _ _ Isomorphism_t
+                (Some (fun i => @OPAQUE _ _ Isomorphism_t None))))
      ; prim_fn := C.mul
      ; model_fn := FM.mul
      ; c_name := "int63_mul"
@@ -251,7 +1104,7 @@ Module UInt63_Proofs.
     props to_Z_properties.
     props add_properties.
     repeat eq_refl_match.
-    rewrite !prim_to_model_to_prim, !model_to_prim_to_model.
+    rewrite !from_to, !to_from.
     unfold FM.to_Z, FM.add, FM.from_Z.
     simpl.
     rewrite Z.mod_small.
@@ -268,7 +1121,7 @@ Module UInt63_Proofs.
     props to_Z_properties.
     props add_properties.
     repeat eq_refl_match.
-    rewrite !prim_to_model_to_prim, !model_to_prim_to_model.
+    rewrite !from_to, !to_from.
     unfold FM.add, FM.from_Z, FM.to_Z.
     simpl.
     rewrite <- !(Z.add_mod y z).
@@ -289,7 +1142,7 @@ Module UInt63_Proofs.
     props add_properties.
     props mul_properties.
     repeat eq_refl_match.
-    rewrite !prim_to_model_to_prim, !model_to_prim_to_model.
+    rewrite !from_to, !to_from.
     unfold FM.mul, FM.add, FM.from_Z, FM.to_Z.
     simpl.
     pose (y' := Z.modulo y (Z.pow_pos 2 63)); fold y'.
@@ -310,7 +1163,7 @@ Module UInt63_Proofs.
     props add_properties.
     props mul_properties.
     repeat eq_refl_match.
-    rewrite !prim_to_model_to_prim, !model_to_prim_to_model.
+    rewrite !from_to, !to_from.
     unfold FM.mul, FM.add, FM.from_Z, FM.to_Z.
     simpl.
     pose (x' := Z.modulo y (Z.pow_pos 2 63)); fold x'.
@@ -412,15 +1265,15 @@ Module Array_Proofs.
 
   Definition Rep_nat : Rep nat. Admitted.
   Definition Rep_t : Rep E.t. Admitted.
-  Axiom Modelled_array : forall {S}, Modelled (C.array S) (FM.array S).
-  Axiom Modelled_ST : forall {S A A'}, Modelled A A' -> Modelled (C.ST S A) (FM.ST S A').
+  Axiom Isomorphism_array : forall {S}, Isomorphism (C.array S) (FM.array S).
+  Axiom Isomorphism_ST : forall {S A A'}, Isomorphism A A' -> Isomorphism (C.ST S A) (FM.ST S A').
 
   Definition pure_ep : extern_properties :=
     {| type_desc :=
       @TYPEPARAM (fun (S : Type) `{Rep_S : Rep S} =>
         @TYPEPARAM (fun (A : Type) `{Rep_A : Rep A} =>
           @TRANSPARENT A Rep_A (Some (fun arr =>
-            @OPAQUE (C.ST S A) (FM.ST S A) (Modelled_ST _) None))))
+            @OPAQUE (C.ST S A) (FM.ST S A) (Isomorphism_ST _) None))))
      ; prim_fn := @C.pure
      ; model_fn := @FM.pure
      ; c_name := "st_pure"
@@ -431,9 +1284,9 @@ Module Array_Proofs.
       @TYPEPARAM (fun (S : Type) `{Rep_S : Rep S} =>
         @TYPEPARAM (fun (A : Type) `{Rep_A : Rep A} =>
           @TYPEPARAM (fun (B : Type) `{Rep_B : Rep B} =>
-            @OPAQUE (C.ST S A) (FM.ST S A) (Modelled_ST _) (Some (fun m =>
-              @OPAQUE (A -> C.ST S B) (A -> FM.ST S B) (Modelled_fn _ (Modelled_ST _)) (Some (fun f =>
-                @OPAQUE (C.ST S B) (FM.ST S B) (Modelled_ST _) None)))))))
+            @OPAQUE (C.ST S A) (FM.ST S A) (Isomorphism_ST _) (Some (fun m =>
+              @OPAQUE (A -> C.ST S B) (A -> FM.ST S B) (Isomorphism_fn _ (Isomorphism_ST _)) (Some (fun f =>
+                @OPAQUE (C.ST S B) (FM.ST S B) (Isomorphism_ST _) None)))))))
      ; prim_fn := @C.bind
      ; model_fn := @FM.bind
      ; c_name := "st_bind"
@@ -443,8 +1296,8 @@ Module Array_Proofs.
     {| type_desc :=
       @TYPEPARAM (fun (A : Type) `{Rep_A : Rep A} =>
           @OPAQUE (forall (S : Type), C.ST S A) (forall (S : Type), FM.ST S A)
-                  (@Modelled_dep_fn Type Type (fun S => C.ST S A) (fun S => FM.ST S A) _
-                                    (fun s s' m => @Modelled_ST _ A A _)) (Some (fun f =>
+                  (@Isomorphism_dep_fn Type Type (fun S => C.ST S A) (fun S => FM.ST S A) _
+                                    (fun s s' m => @Isomorphism_ST _ A A _)) (Some (fun f =>
             @TRANSPARENT A Rep_A None)))
      ; prim_fn := @C.runST
      ; model_fn := @FM.runST
@@ -457,7 +1310,7 @@ Module Array_Proofs.
         @TRANSPARENT nat Rep_nat (Some (fun n =>
           @TRANSPARENT E.t Rep_t (Some (fun a =>
             @OPAQUE (C.ST S (C.array S)) (FM.ST S (FM.array S))
-                    (Modelled_ST Modelled_array) None)))))
+                    (Isomorphism_ST Isomorphism_array) None)))))
      ; prim_fn := @C.new
      ; model_fn := @FM.new
      ; c_name := "array_new"
@@ -466,10 +1319,10 @@ Module Array_Proofs.
   Definition set_ep : extern_properties :=
     {| type_desc :=
       @TYPEPARAM (fun (S : Type) `{Rep_S : Rep S} =>
-        @OPAQUE (C.array S) (FM.array S) Modelled_array (Some (fun arr =>
+        @OPAQUE (C.array S) (FM.array S) Isomorphism_array (Some (fun arr =>
           @TRANSPARENT nat Rep_nat (Some (fun n =>
             @TRANSPARENT E.t Rep_t (Some (fun a =>
-              @OPAQUE (C.ST S unit) (FM.ST S unit) (Modelled_ST _) None)))))))
+              @OPAQUE (C.ST S unit) (FM.ST S unit) (Isomorphism_ST _) None)))))))
      ; prim_fn := @C.set
      ; model_fn := @FM.set
      ; c_name := "array_set"
@@ -478,9 +1331,9 @@ Module Array_Proofs.
   Definition get_ep : extern_properties :=
     {| type_desc :=
       @TYPEPARAM (fun (S : Type) `{Rep_S : Rep S} =>
-        @OPAQUE (C.array S) (FM.array S) Modelled_array (Some (fun arr =>
+        @OPAQUE (C.array S) (FM.array S) Isomorphism_array (Some (fun arr =>
           @TRANSPARENT nat Rep_nat (Some (fun n =>
-            @OPAQUE (C.ST S (option E.t)) (FM.ST S (option E.t)) (Modelled_ST _) None)))))
+            @OPAQUE (C.ST S (option E.t)) (FM.ST S (option E.t)) (Isomorphism_ST _) None)))))
      ; prim_fn := @C.get
      ; model_fn := @FM.get
      ; c_name := "array_get"
@@ -489,8 +1342,8 @@ Module Array_Proofs.
   Definition delete_ep : extern_properties :=
     {| type_desc :=
       @TYPEPARAM (fun (S : Type) `{Rep_S : Rep S} =>
-        @OPAQUE (C.array S) (FM.array S) Modelled_array (Some (fun arr =>
-          @OPAQUE (C.ST S unit) (FM.ST S unit) (Modelled_ST _) None)))
+        @OPAQUE (C.array S) (FM.array S) Isomorphism_array (Some (fun arr =>
+          @OPAQUE (C.ST S unit) (FM.ST S unit) (Isomorphism_ST _) None)))
      ; prim_fn := @C.delete
      ; model_fn := @FM.delete
      ; c_name := "array_delete"
@@ -506,14 +1359,67 @@ Module Array_Proofs.
 
   Ltac prim_rewrites :=
     repeat eq_refl_match;
-    rewrite ?prim_to_model_to_prim, ?model_to_prim_to_model.
+    rewrite ?from_to, ?to_from.
+
+  (* Definition actions_equiv {S A : Type} (x y : FM.ST S A) : Prop := *)
+  (*   forall s, x s = y s. *)
+  (* Set Printing All. *)
+  (* Print actions_equiv. *)
+
+  (* Axiom runST_equiv : forall A (x y : forall (S : Type), FM.ST S A), *)
+  (*     x = y -> *)
+  (*     FM.runST x = FM.runST y. *)
+
+
+  Arguments from A B {_}.
+  Arguments to A B {_}.
+
+  Axiom array_eq : forall S, C.array S = FM.array S.
+  (* Lemma from_eq : *)
+  (*   forall A B x, *)
+  (*     A = B -> *)
+  (*     from A B x = x. *)
+
+  Lemma Isomorphism_FMST {A B : Type} : Isomorphism A B -> Isomorphism (FM.ST unit A) (FM.ST unit B).
+  Proof.
+    intros [f t ft tf].
+    econstructor.
+    Unshelve.
+    3: { intros a x. specialize (a x).
+         exact (f (fst a), (snd a)).}
+    3: { intros a x. specialize (a x).
+         exact (t (fst a), (snd a)).}
+    simpl. intros. apply functional_extensionality. intros. rewrite ?ft, ?tf. destruct (x x0). auto.
+    simpl. intros. apply functional_extensionality. intros. rewrite ?ft, ?tf. destruct (x x0). auto.
+  Defined.
+
+  Lemma from_eq :
+    forall A B x,
+      A = B ->
+      forall (I1 : Isomorphism A B) (I2 : Isomorphism (FM.ST unit B) (FM.ST unit A)),
+        I2 = Isomorphism_sym (Isomorphism_FMST I1) ->
+    (@from A B I1 (fst (@from (FM.ST unit B) (FM.ST unit A) I2 x []))) = fst (x []).
+  Proof.
+    intros A B X eq I1 I2 Ieq.
+    subst.
+  Admitted.
+  (*   unfold fst. *)
+  (*   unfold fst. *)
+  (* Abort. *)
 
   Lemma set_get :
     forall {S : Type} (n len : nat) (bound : n < len) (to_set to_fill : E.t),
-      C.runST (fun _ => C.bind (C.new len to_fill) (fun arr => C.bind (C.set arr n to_set) (fun _ => C.get arr n))) =
-      C.runST (fun _ => C.pure (Some to_set)).
+      (C.runST (fun _ => C.bind (C.new len to_fill) (fun arr => C.bind (C.set arr n to_set) (fun _ => C.get arr n))))
+        =
+      (C.runST (fun _ => C.pure (Some to_set))).
   Proof.
+
+    (* Set Printing Implicit. *)
+    (* Unset Printing Notations. *)
+
+
     intros S n len bound to_set to_fill.
+
     props runST_properties.
     prim_rewrites.
     unfold FM.runST.
@@ -525,68 +1431,77 @@ Module Array_Proofs.
     prim_rewrites.
 
     props bind_properties.
-    props set_properties.
     unfold FM.bind.
+    prim_rewrites.
+
+    props set_properties.
     prim_rewrites.
 
     props get_properties.
     prim_rewrites.
-  Abort.
+
+    unfold fst at 4.
+
+    rewrite !to_sym.
+    rewrite !from_trans.
+
+    rewrite from_eq.
+    rewrite !from_sym.
+    3: {
+      unfold Isomorphism_sym.
+      simpl.
+      Set Printing All.
+      Check (@Isomorphism_ST unit (C.array unit) (C.array unit) (@Isomorphism_refl (C.array unit))).
+      Check (@Isomorphism_refl (FM.ST unit (FM.array unit))).
+      replace (@Isomorphism_ST unit (C.array unit) (C.array unit) (@Isomorphism_refl (C.array unit)))
+         with (@Isomorphism_refl (FM.ST unit (FM.array unit))).
+
+    }
+
+
+
+    Set Printing All.
+
+    (* rewrite array_eq. *)
+
+    (* Set Printing Implicit. *)
+
+    unfold FM.new, FM.set, FM.get.
+    unfold repeat.
+
+    simpl.
+    all: try auto.
+
+
+    rewrite !to_sym.
+    rewrite !from_trans.
+
+
+
+    Unset Printing Implicit.
 
 
     (* rest of the proof is just about the functional model *)
-    (* Set Printing All. *)
-    (* Check (@FM.new unit len to_fill). *)
-    (* Check ((@model_to_prim (C.ST unit (C.array unit)) *)
-    (*                   (FM.ST unit (FM.array unit)) *)
-    (*                   (@Modelled_ST unit (C.array unit) *)
-    (*                      (FM.array unit) (@Modelled_array unit)) *)
-    (*                   (@FM.new unit len to_fill))). *)
-    (* Check ((@prim_to_model (C.ST unit (C.array unit)) *)
-    (*                (FM.ST unit (C.array unit)) *)
-    (*                (@Modelled_ST unit (C.array unit) *)
-    (*                   (C.array unit) *)
-    (*                   (@Modelled_same (C.array unit))) *)
-    (*                (@model_to_prim (C.ST unit (C.array unit)) *)
-    (*                   (FM.ST unit (FM.array unit)) *)
-    (*                   (@Modelled_ST unit (C.array unit) *)
-    (*                      (FM.array unit) (@Modelled_array unit)) *)
-    (*                   (@FM.new unit len to_fill)) *)
-    (*                (@nil (list E.t)))). *)
-    (* Check (((@prim_to_model (C.array unit) (FM.array unit) *)
-    (*          (@Modelled_array unit) *)
-    (*          (@fst (C.array unit) FM.arrays *)
-    (*             (@prim_to_model (C.ST unit (C.array unit)) *)
-    (*                (FM.ST unit (C.array unit)) *)
-    (*                (@Modelled_ST unit (C.array unit) *)
-    (*                   (C.array unit) *)
-    (*                   (@Modelled_same (C.array unit))) *)
-    (*                (@model_to_prim (C.ST unit (C.array unit)) *)
-    (*                   (FM.ST unit (FM.array unit)) *)
-    (*                   (@Modelled_ST unit (C.array unit) *)
-    (*                      (FM.array unit) (@Modelled_array unit)) *)
-    (*                   (@FM.new unit len to_fill)) *)
-    (*                (@nil (list E.t))))))). *)
+    Set Printing All.
+    Check (@FM.new unit len to_fill).
+    rewrite ?from_to, ?to_from.
+    unfold FM.new.
+    rewrite ?from_to, ?to_from.
 
-    (* rewrite ?prim_to_model_to_prim, ?model_to_prim_to_model. *)
-    (* Check (@model_to_prim_to_model (C.ST unit (C.array unit)) (FM.ST unit (FM.array unit)) (@Modelled_ST unit (C.array unit) (FM.array unit) (@Modelled_array unit))). *)
-    (* unfold FM.new. *)
-    (* rewrite ?prim_to_model_to_prim, ?model_to_prim_to_model. *)
+    unfold from.
 
-    (* unfold model_to_prim. *)
-
-    (* assert (forall (x : FM.ST S nat), prim_to_model (model_to_prim x) = x). *)
-    (* intros. prim_rewrites. auto. *)
+    assert (forall (x : FM.ST S nat), to (from x) = x).
+    intros. prim_rewrites. auto.
 
 
-    (* rewrite (H (fun s : FM.arrays => (length s, s ++ [repeat to_fill len]))). *)
-    (* rewrite !model_to_prim_to_model. *)
-    (* unfold FM.get, FM.set, FM.new. *)
-    (* simpl. *)
-    (* prim_rewrites. *)
+    rewrite (H (fun s : FM.arrays => (length s, s ++ [repeat to_fill len]))).
+    rewrite !to_from.
+    unfold FM.get, FM.set, FM.new.
+    simpl.
+    prim_rewrites.
 
 
-  (* Qed. *)
+  Qed.
 
 End Array_Proofs.
 
